Tap

Refinery/Term/Extrinsic/Wf/Rewrite.lean
@@ -7,7 +7,7 @@ namespace Refinery
 namespace Term
 
 variable  {φ : Type u} {α : Type v} {ε : Type w} [S : Signature φ α ε]
-          {R : DRWS φ α} [R.UWkCongr]
+          {R : DRWS φ α}
 
 def Wf.eqv.equivFwdStep
   {Γ : Ctx? α} {A : Ty α} (a b : Wf R Γ A) (h : (DRWS.EquivFwdStep (S := S)).rel a.deriv b.deriv)
@@ -16,7 +16,84 @@ def Wf.eqv.equivFwdStep
     .base (.equiv (.bwd h)),
   ⟩
 
-def Eqv.let_op {Γ Γl Γr : Ctx? α} {f A B C}
+--TODO: backwards rules, with hax... that autocompleted to haxioms.
+
+theorem Eqv.bind_op {Γ : Ctx? α} {f A B}
+  (hf : S.FnTy f A B) (a : Eqv R Γ A)
+  : a.op hf
+    = a.let₁ Γ.erase_left (.op hf .bv0) := by
+  induction a using quotInd
+  apply sound
+  apply Wf.eqv.equivFwdStep
+  apply DRWS.EquivFwdStep.let_bind
+  apply DRWS.LetBind.bind_op
+
+theorem Eqv.terminal {Γ : Ctx? α} (a : Eqv R Γ Ty.unit)
+  : (a.let₁ Γ.erase_left (.unit _))
+  = a := by
+  induction a using quotInd
+  apply sound
+  apply Wf.eqv.equivFwdStep
+  apply DRWS.EquivFwdStep.step
+  apply DRWS.Step.terminal
+
+theorem Eqv.initial {Γ Γl Γr : Ctx? α} {B}
+  (hΓ : Γ.SSplit Γl Γr)
+  (a : Eqv R Γr Ty.empty)
+  (b c : Eqv R (Γl.cons ⟨Ty.empty, ⊤⟩) B)
+  : a.let₁ hΓ b = a.let₁ hΓ c := by
+  induction a, b, c using quotInd₃
+  apply sound
+  apply Wf.eqv.equivFwdStep
+  apply DRWS.EquivFwdStep.step
+  apply DRWS.Step.initial
+
+theorem Eqv.let₂_eta {Γ : Ctx? α} {A B : Ty α}
+  (a : Eqv R Γ (A.tensor B))
+  : a.let₂ Γ.erase_left (.pair (((Γ.erase.both).cons (.left _)).cons (.right _)) .bv1 .bv0)
+  = a := by
+  induction a using quotInd
+  apply sound
+  apply Wf.eqv.equivFwdStep
+  apply DRWS.EquivFwdStep.step
+  apply DRWS.Step.let₂_eta
+
+theorem Eqv.case_eta {Γ : Ctx? α} {A B : Ty α}
+  (a : Eqv R Γ (A.coprod B))
+  : a.case Γ.erase_left (.inl _ _ .bv0) (.inr _ _ .bv0) = a := by
+  induction a using quotInd
+  apply sound
+  apply Wf.eqv.equivFwdStep
+  apply DRWS.EquivFwdStep.step
+  apply DRWS.Step.case_eta
+
+theorem Eqv.case_inl {Γ Γl Γr : Ctx? α} {A B C}
+  (hΓ : Γ.SSplit Γl Γr)
+  (a : Eqv R Γr A)
+  (b : Eqv R (Γl.cons ⟨A, ⊤⟩) C)
+  (c : Eqv R (Γl.cons ⟨B, ⊤⟩) C)
+  : ((a.inl _ _).case hΓ b c) = a.let₁ hΓ b := by
+  induction a, b, c using quotInd₃
+  apply sound
+  apply Wf.eqv.equivFwdStep
+  apply DRWS.EquivFwdStep.step
+  apply DRWS.Step.case_inl
+
+theorem Eqv.case_inr {Γ Γl Γr : Ctx? α} {A B C}
+  (hΓ : Γ.SSplit Γl Γr)
+  (a : Eqv R Γr B)
+  (b : Eqv R (Γl.cons ⟨A, ⊤⟩) C)
+  (c : Eqv R (Γl.cons ⟨B, ⊤⟩) C)
+  : ((a.inr _ _).case hΓ b c) = a.let₁ hΓ c := by
+  induction a, b, c using quotInd₃
+  apply sound
+  apply Wf.eqv.equivFwdStep
+  apply DRWS.EquivFwdStep.step
+  apply DRWS.Step.case_inr
+
+variable [R.UWkCongr]
+
+theorem Eqv.let_op {Γ Γl Γr : Ctx? α} {f A B C}
     (hΓ : Γ.SSplit Γl Γr) (hf : S.FnTy f A B) (a : Eqv R Γr A) (b : Eqv R (Γl.cons ⟨B, ⊤⟩) C)
     : (a.op hf).let₁ hΓ b
     = a.let₁ hΓ (.let₁ (Γl.erase_right.cons (.right _)) (.op hf .bv0) (b.wk1 _)) := by
@@ -26,7 +103,7 @@ def Eqv.let_op {Γ Γl Γr : Ctx? α} {f A B C}
   apply DRWS.EquivFwdStep.let_move
   apply DRWS.LetMove.let_op
 
-def Eqv.let_let₁ {Γ Γl Γc Γm Γr : Ctx? α} {A B C}
+theorem Eqv.let_let₁ {Γ Γl Γc Γm Γr : Ctx? α} {A B C}
     (hΓ : Γ.SSplit Γl Γc) (hΓc : Γc.SSplit Γm Γr)
     (a : Eqv R Γr A) (b : Eqv R (Γm.cons ⟨A, ⊤⟩) B) (c : Eqv R (Γl.cons ⟨B, ⊤⟩) C)
     : (a.let₁ hΓc b).let₁ hΓ c
@@ -37,7 +114,7 @@ def Eqv.let_let₁ {Γ Γl Γc Γm Γr : Ctx? α} {A B C}
   apply DRWS.EquivFwdStep.let_move
   apply DRWS.LetMove.let_let₁
 
-def Eqv.let_let₂ {Γ Γl Γc Γm Γr : Ctx? α} {A B C D}
+theorem Eqv.let_let₂ {Γ Γl Γc Γm Γr : Ctx? α} {A B C D}
     (hΓ : Γ.SSplit Γl Γc) (hΓc : Γc.SSplit Γm Γr)
     (a : Eqv R Γr (A.tensor B)) (b : Eqv R ((Γm.cons ⟨A, ⊤⟩).cons ⟨B, ⊤⟩) C) (c : Eqv R (Γl.cons ⟨C, ⊤⟩) D)
     : (a.let₂ hΓc b).let₁ hΓ c
@@ -49,7 +126,7 @@ def Eqv.let_let₂ {Γ Γl Γc Γm Γr : Ctx? α} {A B C D}
   apply DRWS.EquivFwdStep.let_move
   apply DRWS.LetMove.let_let₂
 
-def Eqv.let_case {Γ Γl Γc Γm Γr : Ctx? α} {A B C D}
+theorem Eqv.let_case {Γ Γl Γc Γm Γr : Ctx? α} {A B C D}
     (hΓ : Γ.SSplit Γl Γc) (hΓc : Γc.SSplit Γm Γr)
     (a : Eqv R Γr (A.coprod B)) (b : Eqv R (Γm.cons ⟨A, ⊤⟩) C)
     (c : Eqv R (Γm.cons ⟨B, ⊤⟩) C) (d : Eqv R (Γl.cons ⟨C, ⊤⟩) D)
@@ -62,20 +139,7 @@ def Eqv.let_case {Γ Γl Γc Γm Γr : Ctx? α} {A B C D}
   apply DRWS.EquivFwdStep.let_move
   apply DRWS.LetMove.let_case
 
---TODO: backwards rules, with hax... that autocompleted to haxioms.
-
-def Eqv.bind_op {Γ : Ctx? α} {f A B}
-  (hf : S.FnTy f A B) (a : Eqv R Γ A)
-  : a.op hf
-    = a.let₁ Γ.erase_left (.op hf .bv0) := by
-  induction a using quotInd
-  apply sound
-  apply Wf.eqv.equivFwdStep
-  apply DRWS.EquivFwdStep.let_bind
-  apply DRWS.LetBind.bind_op
-
-
-def Eqv.bind_let₂ {Γ Γl Γr : Ctx? α} {A B C}
+theorem Eqv.bind_let₂ {Γ Γl Γr : Ctx? α} {A B C}
   (hΓ : Γ.SSplit Γl Γr)
   (a : Eqv R Γr (A.tensor B))
   (b : Eqv R ((Γl.cons ⟨A, ⊤⟩).cons ⟨B, ⊤⟩) C)
@@ -87,7 +151,7 @@ def Eqv.bind_let₂ {Γ Γl Γr : Ctx? α} {A B C}
   apply DRWS.EquivFwdStep.let_bind
   apply DRWS.LetBind.bind_let₂
 
-def Eqv.bind_case {Γ Γl Γr : Ctx? α} {A B C}
+theorem Eqv.bind_case {Γ Γl Γr : Ctx? α} {A B C}
   (hΓ : Γ.SSplit Γl Γr)
   (a : Eqv R Γr (A.coprod B))
   (b : Eqv R (Γl.cons ⟨A, ⊤⟩) C)
@@ -100,7 +164,7 @@ def Eqv.bind_case {Γ Γl Γr : Ctx? α} {A B C}
   apply DRWS.EquivFwdStep.let_bind
   apply DRWS.LetBind.bind_case
 
-def Eqv.bind_iter {Γ Γl Γr : Ctx? α} {A B : Ty α}
+theorem Eqv.bind_iter {Γ Γl Γr : Ctx? α} {A B : Ty α}
   (hΓ : Γ.SSplit Γl Γr) (hc : Γl.copy) (hd : Γl.del)
   (a : Eqv R Γr A)
   (b : Eqv R (Γl.cons ⟨A, ⊤⟩) (B.coprod A))
@@ -112,46 +176,7 @@ def Eqv.bind_iter {Γ Γl Γr : Ctx? α} {A B : Ty α}
   apply DRWS.EquivFwdStep.let_bind
   apply DRWS.LetBind.bind_iter
 
-def Eqv.terminal {Γ : Ctx? α} (a : Eqv R Γ Ty.unit)
-  : (a.let₁ Γ.erase_left (.unit _))
-  = a := by
-  induction a using quotInd
-  apply sound
-  apply Wf.eqv.equivFwdStep
-  apply DRWS.EquivFwdStep.step
-  apply DRWS.Step.terminal
-
-def Eqv.initial {Γ Γl Γr : Ctx? α} {B}
-  (hΓ : Γ.SSplit Γl Γr)
-  (a : Eqv R Γr Ty.empty)
-  (b c : Eqv R (Γl.cons ⟨Ty.empty, ⊤⟩) B)
-  : a.let₁ hΓ b = a.let₁ hΓ c := by
-  induction a, b, c using quotInd₃
-  apply sound
-  apply Wf.eqv.equivFwdStep
-  apply DRWS.EquivFwdStep.step
-  apply DRWS.Step.initial
-
-def Eqv.let₂_eta {Γ : Ctx? α} {A B : Ty α}
-  (a : Eqv R Γ (A.tensor B))
-  : a.let₂ Γ.erase_left (.pair (((Γ.erase.both).cons (.left _)).cons (.right _)) .bv1 .bv0)
-  = a := by
-  induction a using quotInd
-  apply sound
-  apply Wf.eqv.equivFwdStep
-  apply DRWS.EquivFwdStep.step
-  apply DRWS.Step.let₂_eta
-
-def Eqv.case_eta {Γ : Ctx? α} {A B : Ty α}
-  (a : Eqv R Γ (A.coprod B))
-  : a.case Γ.erase_left (.inl _ _ .bv0) (.inr _ _ .bv0) = a := by
-  induction a using quotInd
-  apply sound
-  apply Wf.eqv.equivFwdStep
-  apply DRWS.EquivFwdStep.step
-  apply DRWS.Step.case_eta
-
-def Eqv.let₂_beta {Γ Γc Γl Γm Γr : Ctx? α} {A B C}
+theorem Eqv.let₂_beta {Γ Γc Γl Γm Γr : Ctx? α} {A B C}
   (hΓ : Γ.SSplit Γl Γc) (hΓc : Γc.SSplit Γm Γr)
   (a : Eqv R Γm A) (b : Eqv R Γr B)
   (c : Eqv R ((Γl.cons ⟨A, ⊤⟩).cons ⟨B, ⊤⟩) C)
@@ -181,31 +206,7 @@ theorem Eqv.let₂_beta_anti {Γ Γc Γl Γm Γr : Ctx? α} {A B C}
   rfl
   rfl
 
-def Eqv.case_inl {Γ Γl Γr : Ctx? α} {A B C}
-  (hΓ : Γ.SSplit Γl Γr)
-  (a : Eqv R Γr A)
-  (b : Eqv R (Γl.cons ⟨A, ⊤⟩) C)
-  (c : Eqv R (Γl.cons ⟨B, ⊤⟩) C)
-  : ((a.inl _ _).case hΓ b c) = a.let₁ hΓ b := by
-  induction a, b, c using quotInd₃
-  apply sound
-  apply Wf.eqv.equivFwdStep
-  apply DRWS.EquivFwdStep.step
-  apply DRWS.Step.case_inl
-
-def Eqv.case_inr {Γ Γl Γr : Ctx? α} {A B C}
-  (hΓ : Γ.SSplit Γl Γr)
-  (a : Eqv R Γr B)
-  (b : Eqv R (Γl.cons ⟨A, ⊤⟩) C)
-  (c : Eqv R (Γl.cons ⟨B, ⊤⟩) C)
-  : ((a.inr _ _).case hΓ b c) = a.let₁ hΓ c := by
-  induction a, b, c using quotInd₃
-  apply sound
-  apply Wf.eqv.equivFwdStep
-  apply DRWS.EquivFwdStep.step
-  apply DRWS.Step.case_inr
-
-def Eqv.fixpoint {Γ Γl Γr : Ctx? α} {A B : Ty α}
+theorem Eqv.fixpoint {Γ Γl Γr : Ctx? α} {A B : Ty α}
   (hΓ : Γ.SSplit Γl Γr) (hc : Γl.copy) (hd : Γl.del)
   (a : Eqv R Γr A)
   (b : Eqv R (Γl.cons ⟨A, ⊤⟩) (B.coprod A))
@@ -218,7 +219,7 @@ def Eqv.fixpoint {Γ Γl Γr : Ctx? α} {A B : Ty α}
   apply DRWS.EquivFwdStep.step
   apply DRWS.Step.fixpoint
 
-def Eqv.codiag {Γ Γl Γr : Ctx? α} {A B : Ty α}
+theorem Eqv.codiag {Γ Γl Γr : Ctx? α} {A B : Ty α}
   (hΓ : Γ.SSplit Γl Γr) (hc : Γl.copy) (hd : Γl.del)
   (a : Eqv R Γr A)
   (b : Eqv R (Γl.cons ⟨A, ⊤⟩) ((B.coprod A).coprod A))
